Std/Data/List/Lemmas.lean
@@ -9,6 +9,7 @@ import Std.Data.List.Basic
 import Std.Data.Option.Lemmas
 import Std.Classes.BEq
 import Std.Tactic.Ext
+import Std.Tactic.Simpa
 
 namespace List
 
@@ -215,9 +216,6 @@ theorem forall_mem_nil (p : α → Prop) : ∀ x ∈ @nil α, p x := fun.
 
 theorem exists_mem_cons {p : α → Prop} {a : α} {l : List α} :
     (∃ x ∈ a :: l, p x) ↔ p a ∨ ∃ x ∈ l, p x := by simp
-
-theorem forall_mem_cons {p : α → Prop} {a : α} {l : List α} :
-    (∀ x ∈ a :: l, p x) ↔ p a ∧ ∀ x ∈ l, p x := by simp
 
 theorem forall_mem_singleton {p : α → Prop} {a : α} : (∀ x ∈ [a], p x) ↔ p a := by
   simp only [mem_singleton, forall_eq]
@@ -1768,3 +1766,194 @@ theorem disjoint_take_drop : ∀ {l : List α}, l.Nodup → m ≤ n → Disjoint
     ∀ (l : List α), takeWhile p l ++ dropWhile p l = l
   | [] => rfl
   | x :: xs => by simp [takeWhile, dropWhile]; cases p x <;> simp [takeWhile_append_dropWhile p xs]
+
+/-! ### Chain -/
+
+--Porting note: attribute in Lean3, but not in Lean4 Std so added here instead
+attribute [simp] Chain.nil
+
+@[simp]
+theorem chain_cons {a b : α} {l : List α} : Chain R a (b :: l) ↔ R a b ∧ Chain R b l :=
+  ⟨fun p ↦ by cases p with | cons n p => exact ⟨n, p⟩,
+   fun ⟨n, p⟩ ↦ p.cons n⟩
+
+theorem rel_of_chain_cons {a b : α} {l : List α} (p : Chain R a (b :: l)) : R a b :=
+  (chain_cons.1 p).1
+
+theorem chain_of_chain_cons {a b : α} {l : List α} (p : Chain R a (b :: l)) : Chain R b l :=
+  (chain_cons.1 p).2
+
+theorem Chain.imp' {R S : α → α → Prop} (HRS : ∀ ⦃a b⦄, R a b → S a b) {a b : α}
+    (Hab : ∀ ⦃c⦄, R a c → S b c) {l : List α} (p : Chain R a l) : Chain S b l := by
+  induction p generalizing b with
+  | nil => constructor
+  | cons r _ ih =>
+    constructor
+    · exact Hab r
+    · exact ih (@HRS _)
+
+theorem Chain.imp {R S : α → α → Prop} (H : ∀ a b, R a b → S a b) {a : α} {l : List α}
+    (p : Chain R a l) : Chain S a l :=
+  p.imp' H (H a)
+
+protected theorem Pairwise.chain (p : Pairwise R (a :: l)) : Chain R a l := by
+  let ⟨r, p'⟩ := pairwise_cons.1 p; clear p
+  induction p' generalizing a with
+  | nil => exact Chain.nil
+  | @cons b l r' _ IH =>
+    simp only [chain_cons, forall_mem_cons] at r
+    exact chain_cons.2 ⟨r.1, IH r'⟩
+
+/-! ### range', range -/
+
+@[simp] theorem length_range' (s step) : ∀ n : Nat, length (range' s n step) = n
+  | 0 => rfl
+  | _ + 1 => congrArg succ (length_range' _ _ _)
+
+@[simp] theorem range'_eq_nil : range' s n step = [] ↔ n = 0 := by
+  rw [← length_eq_zero, length_range']
+
+theorem mem_range' : ∀{n}, m ∈ range' s n step ↔ ∃ i < n, m = s + step * i
+  | 0 => by simp [range', Nat.not_lt_zero]
+  | n + 1 => by
+    have h (i) : i ≤ n ↔ i = 0 ∨ ∃ j, i = succ j ∧ j < n := by cases i <;> simp [Nat.succ_le]
+    simp [range', mem_range', Nat.lt_succ, h]; simp only [← exists_and_right, and_assoc]
+    rw [exists_comm]; simp [Nat.mul_succ, Nat.add_assoc, Nat.add_comm]
+
+@[simp] theorem mem_range'_1 : m ∈ range' s n ↔ s ≤ m ∧ m < s + n := by
+  simp [mem_range']; exact ⟨
+    fun ⟨i, h, e⟩ => e ▸ ⟨Nat.le_add_right .., Nat.add_lt_add_left h _⟩,
+    fun ⟨h₁, h₂⟩ => ⟨m - s, Nat.sub_lt_left_of_lt_add h₁ h₂, (Nat.add_sub_cancel' h₁).symm⟩⟩
+
+theorem map_add_range' (a) : ∀ s n step, map (a + ·) (range' s n step) = range' (a + s) n step
+  | _, 0, _ => rfl
+  | s, n + 1, step => by simp [range', map_add_range' _ (s + step) n step, Nat.add_assoc]
+
+theorem map_sub_range' (a s n : Nat) (h : a ≤ s) :
+    map (· - a) (range' s n step) = range' (s - a) n step := by
+  conv => lhs; rw [← Nat.add_sub_cancel' h]
+  rw [← map_add_range', map_map, (?_ : _∘_ = _), map_id]
+  funext x; apply Nat.add_sub_cancel_left
+
+theorem chain_succ_range' : ∀ s n step : Nat,
+    Chain (fun a b => b = a + step) s (range' (s + step) n step)
+  | _, 0, _ => Chain.nil
+  | s, n + 1, step => (chain_succ_range' (s + step) n step).cons rfl
+
+theorem chain_lt_range' (s n : Nat) {step} (h : 0 < step) :
+    Chain (· < ·) s (range' (s + step) n step) :=
+  (chain_succ_range' s n step).imp fun _ _ e => e.symm ▸ Nat.lt_add_of_pos_right h
+
+theorem range'_append : ∀ s m n step : Nat,
+    range' s m step ++ range' (s + step * m) n step = range' s (n + m) step
+  | s, 0, n, step => rfl
+  | s, m + 1, n, step => by
+    simpa [range', Nat.mul_succ, Nat.add_assoc, Nat.add_comm]
+      using range'_append (s + step) m n step
+
+@[simp] theorem range'_append_1 (s m n : Nat) :
+    range' s m ++ range' (s + m) n = range' s (n + m) := by simpa using range'_append s m n 1
+
+theorem range'_sublist_right {s m n : Nat} : range' s m step <+ range' s n step ↔ m ≤ n :=
+  ⟨fun h => by simpa only [length_range'] using h.length_le,
+   fun h => by rw [← Nat.sub_add_cancel h, ← range'_append]; apply sublist_append_left⟩
+
+theorem range'_subset_right {s m n : Nat} (step0 : 0 < step) :
+    range' s m step ⊆ range' s n step ↔ m ≤ n := by
+  refine ⟨fun h => Nat.le_of_not_lt fun hn => ?_, fun h => (range'_sublist_right.2 h).subset⟩
+  have ⟨i, h', e⟩ := mem_range'.1 <| h <| mem_range'.2 ⟨_, hn, rfl⟩
+  exact Nat.ne_of_gt h' (Nat.eq_of_mul_eq_mul_left step0 (Nat.add_left_cancel e))
+
+theorem range'_subset_right_1 {s m n : Nat} : range' s m ⊆ range' s n ↔ m ≤ n :=
+  range'_subset_right (by decide)
+
+theorem get?_range' (s step) : ∀ {m n : Nat}, m < n → get? (range' s n step) m = some (s + step * m)
+  | 0, n + 1, _ => rfl
+  | m + 1, n + 1, h =>
+    (get?_range' (s + step) step (Nat.lt_of_add_lt_add_right h)).trans <| by
+      simp [Nat.mul_succ, Nat.add_assoc, Nat.add_comm]
+
+@[simp] theorem get_range' {n m step} (i) (H : i < (range' n m step).length) :
+    get (range' n m step) ⟨i, H⟩ = n + step * i :=
+  (get?_eq_some.1 <| get?_range' n step (by simpa using H)).2
+
+theorem range'_concat (s n : Nat) : range' s (n + 1) step = range' s n step ++ [s + step * n] := by
+  rw [Nat.add_comm n 1]; exact (range'_append s n 1 step).symm
+
+theorem range'_1_concat (s n : Nat) : range' s (n + 1) = range' s n ++ [s + n] := by
+  simp [range'_concat]
+
+theorem range_loop_range' : ∀ s n : Nat, range.loop s (range' s n) = range' 0 (n + s)
+  | 0, n => rfl
+  | s + 1, n => by rw [← Nat.add_assoc, Nat.add_right_comm n s 1]; exact range_loop_range' s (n + 1)
+
+theorem range_eq_range' (n : Nat) : range n = range' 0 n :=
+  (range_loop_range' n 0).trans <| by rw [Nat.zero_add]
+
+theorem range_succ_eq_map (n : Nat) : range (n + 1) = 0 :: map succ (range n) := by
+  rw [range_eq_range', range_eq_range', range', Nat.add_comm, ← map_add_range']
+  congr; exact funext one_add
+
+theorem range'_eq_map_range (s n : Nat) : range' s n = map (s + ·) (range n) := by
+  rw [range_eq_range', map_add_range']; rfl
+
+@[simp] theorem length_range (n : Nat) : length (range n) = n := by
+  simp only [range_eq_range', length_range']
+
+@[simp] theorem range_eq_nil {n : Nat} : range n = [] ↔ n = 0 := by
+  rw [← length_eq_zero, length_range]
+
+theorem range_sublist {m n : Nat} : range m <+ range n ↔ m ≤ n := by
+  simp only [range_eq_range', range'_sublist_right]
+
+theorem range_subset {m n : Nat} : range m ⊆ range n ↔ m ≤ n := by
+  simp only [range_eq_range', range'_subset_right]
+
+@[simp]
+theorem mem_range {m n : Nat} : m ∈ range n ↔ m < n := by
+  simp only [range_eq_range', mem_range'_1, Nat.zero_le, true_and, Nat.zero_add]
+
+theorem not_mem_range_self {n : Nat} : n ∉ range n := by simp
+
+theorem self_mem_range_succ (n : Nat) : n ∈ range (n + 1) := by simp
+
+theorem get?_range {m n : Nat} (h : m < n) : get? (range n) m = some m := by
+  simp [range_eq_range', get?_range' _ _ h]
+
+theorem range_succ (n : Nat) : range (succ n) = range n ++ [n] := by
+  simp only [range_eq_range', range'_1_concat, Nat.zero_add]
+
+@[simp] theorem range_zero : range 0 = [] := rfl
+
+theorem range_add (a b : Nat) : range (a + b) = range a ++ (range b).map (a + ·) := by
+  rw [← range'_eq_map_range]
+  simpa [range_eq_range', Nat.add_comm] using (range'_append_1 0 a b).symm
+
+theorem iota_eq_reverse_range' : ∀ n : Nat, iota n = reverse (range' 1 n)
+  | 0 => rfl
+  | n + 1 => by simp [iota, range'_concat, iota_eq_reverse_range' n, reverse_append, Nat.add_comm]
+
+@[simp] theorem length_iota (n : Nat) : length (iota n) = n := by simp [iota_eq_reverse_range']
+
+theorem mem_iota {m n : Nat} : m ∈ iota n ↔ 1 ≤ m ∧ m ≤ n := by
+  simp [iota_eq_reverse_range', Nat.add_comm, Nat.lt_succ]
+
+theorem reverse_range' : ∀ s n : Nat, reverse (range' s n) = map (s + n - 1 - ·) (range n)
+  | s, 0 => rfl
+  | s, n + 1 => by
+    rw [range'_1_concat, reverse_append, range_succ_eq_map,
+      show s + (n + 1) - 1 = s + n from rfl, map, map_map]
+    simp [reverse_range', Nat.sub_right_comm]; rfl
+
+@[simp] theorem get_range {n} (i) (H : i < (range n).length) : get (range n) ⟨i, H⟩ = i :=
+  Option.some.inj <| by rw [← get?_eq_get _, get?_range (by simpa using H)]
+
+/-! ### enum, enumFrom -/
+
+@[simp] theorem enumFrom_map_fst (n) :
+    ∀ (l : List α), map Prod.fst (enumFrom n l) = range' n l.length
+  | [] => rfl
+  | _ :: _ => congrArg (cons _) (enumFrom_map_fst _ _)
+
+@[simp] theorem enum_map_fst (l : List α) : map Prod.fst (enum l) = range l.length := by
+  simp only [enum, enumFrom_map_fst, range_eq_range']
