Std/Data/Nat/Lemmas.lean
@@ -388,6 +388,9 @@ protected theorem le_or_le (a b : Nat) : a ≤ b ∨ b ≤ a := (Nat.lt_or_ge _ 
 protected theorem lt_or_eq_of_le {n m : Nat} (h : n ≤ m) : n < m ∨ n = m :=
   (Nat.lt_or_ge _ _).imp_right (Nat.le_antisymm h)
 
+protected theorem le_iff_lt_or_eq {n m : Nat} : n ≤ m ↔ n < m ∨ n = m :=
+  ⟨Nat.lt_or_eq_of_le, (·.elim Nat.le_of_lt Nat.le_of_eq)⟩
+
 theorem le_zero {i : Nat} : i ≤ 0 ↔ i = 0 :=
   ⟨Nat.eq_zero_of_le_zero, fun h => h ▸ Nat.le_refl i⟩
 
@@ -408,7 +411,7 @@ protected theorem sub_le_sub_left (k : Nat) (h : n ≤ m) : k - m ≤ k - n :=
 theorem succ_sub_sub_succ (n m k : Nat) : succ n - m - succ k = n - m - k := by
   rw [Nat.sub_sub, Nat.sub_sub, add_succ, succ_sub_succ]
 
-protected theorem sub.right_comm (m n k : Nat) : m - n - k = m - k - n := by
+protected theorem sub_right_comm (m n k : Nat) : m - n - k = m - k - n := by
   rw [Nat.sub_sub, Nat.sub_sub, Nat.add_comm]
 
 protected theorem mul_self_sub_mul_self_eq (a b : Nat) : a * a - b * b = (a + b) * (a - b) := by
